Slight clean-up of SUM_SET work.  In particular, there's a general result possible justifying recursion equations that look like:     ITSET f (x INSERT s) b = f x (ITSET f s b) This is the FOLDR version, as opposed to the FOLDL version, or the recursing version rather than the accumulator version.   Also define functions to get the minimum and maximum elements of sets of numbers.  The former is just the LEAST quantifier.  (Just realised that perhaps shouldn't even have a new constant for MIN_SET; could do it with overloading; but then the pretty-printing system would pick one or the other to be "the way" to print that constant, which could be confusing too.  Dunno.

src/pred_set/src/pred_setScript.sml
@@ -2969,8 +2969,8 @@ val ITSET_INSERT = store_thm(
 val absorption = #1 (EQ_IMP_RULE (SPEC_ALL ABSORPTION))
 val delete_non_element = #1 (EQ_IMP_RULE (SPEC_ALL DELETE_NON_ELEMENT))
 
-val AC_ITSET_INSERT = store_thm(
-  "AC_ITSET_INSERT",
+val COMMUTING_ITSET_INSERT = store_thm(
+  "COMMUTING_ITSET_INSERT",
   ``!f s. (!x y z. f x (f y z) = f y (f x z)) /\
           FINITE s ==>
           !x b. ITSET f (x INSERT s) b = ITSET f (s DELETE x) (f x b)``,
@@ -3026,11 +3026,26 @@ val AC_ITSET_INSERT = store_thm(
      (FULL_SIMP_TAC bool_ss [EXTENSION, IN_INSERT] THEN PROVE_TAC []) THEN
   ASM_SIMP_TAC arith_ss [delete_non_element]);
 
+val COMMUTING_ITSET_RECURSES = store_thm(
+  "COMMUTING_ITSET_RECURSES",
+  ``!f e s b. (!x y z. f x (f y z) = f y (f x z)) /\ FINITE s ==>
+              (ITSET f (e INSERT s) b = f e (ITSET f (s DELETE e) b))``,
+  Q_TAC SUFF_TAC
+    `!f. (!x y z. f x (f y z) = f y (f x z)) ==>
+         !s. FINITE s ==>
+             !e b. ITSET f (e INSERT s) b = f e (ITSET f (s DELETE e) b)` THEN1
+    PROVE_TAC [] THEN
+  GEN_TAC THEN STRIP_TAC THEN
+  ASM_SIMP_TAC (srw_ss()) [COMMUTING_ITSET_INSERT] THEN
+  Q_TAC SUFF_TAC
+    `!s. FINITE s ==> !e b. ITSET f s (f e b) = f e (ITSET f s b)` THEN1
+    PROVE_TAC [FINITE_DELETE] THEN
+  HO_MATCH_MP_TAC FINITE_INDUCT THEN CONJ_TAC THENL [
+    SIMP_TAC bool_ss [ITSET_THM, FINITE_EMPTY],
+    ASM_SIMP_TAC bool_ss [COMMUTING_ITSET_INSERT, delete_non_element]
+  ]);
 
-
-val SUM_SET_def = new_definition(
-  "SUM_SET_def",
-  ``SUM_SET s = ITSET (+) s 0``);
+val SUM_SET_def = new_definition("SUM_SET_def", ``SUM_SET s = ITSET (+) s 0``);
 
 val SUM_SET_THM = store_thm(
   "SUM_SET_THM",
@@ -3038,18 +3053,7 @@ val SUM_SET_THM = store_thm(
     (!x s. FINITE s ==> (SUM_SET (x INSERT s) = x + SUM_SET (s DELETE x)))``,
   CONJ_TAC THEN REWRITE_TAC [SUM_SET_def] THENL [
     SIMP_TAC bool_ss [FINITE_EMPTY, ITSET_THM],
-    ASSUME_TAC (SIMP_RULE arith_ss [] (Q.ISPEC `(+)` AC_ITSET_INSERT)) THEN
-    ASM_SIMP_TAC arith_ss [] THEN
-    Q_TAC SUFF_TAC
-      `!s. FINITE s ==>
-           !x n. ITSET (+) s (x + n) = x + ITSET (+) s n` THEN1
-      PROVE_TAC [ADD_CLAUSES, FINITE_DELETE] THEN
-    HO_MATCH_MP_TAC FINITE_INDUCT THEN CONJ_TAC THENL [
-      SIMP_TAC bool_ss [ITSET_THM, FINITE_EMPTY],
-      REPEAT STRIP_TAC THEN
-      ASM_SIMP_TAC bool_ss [delete_non_element] THEN
-      REWRITE_TAC [ADD_ASSOC]
-    ]
+    PROVE_TAC [SIMP_RULE arith_ss [] (Q.ISPEC `(+)` COMMUTING_ITSET_RECURSES)]
   ]);
 
 val SUM_SET_SING = store_thm(
@@ -3146,9 +3150,92 @@ val SUM_SET_UNION = store_thm(
   ]);
 
 
+val max_lemma = prove(
+  ``!s. FINITE s ==> ~(s = {}) ==> ?x. x IN s /\ !y. y IN s ==> y <= x``,
+  HO_MATCH_MP_TAC FINITE_INDUCT THEN
+  SIMP_TAC bool_ss [NOT_INSERT_EMPTY, IN_INSERT] THEN
+  REPEAT STRIP_TAC THEN
+  Q.ISPEC_THEN `s` STRIP_ASSUME_TAC SET_CASES THENL [
+    ASM_SIMP_TAC arith_ss [NOT_IN_EMPTY],
+    `~(s = {})` by PROVE_TAC [NOT_INSERT_EMPTY] THEN
+    `?m. m IN s /\ !y. y IN s ==> y <= m` by PROVE_TAC [] THEN
+    Cases_on `e <= m` THENL [
+      PROVE_TAC [],
+      `m <= e` by RW_TAC arith_ss [] THEN
+      PROVE_TAC [LESS_EQ_REFL, LESS_EQ_TRANS]
+    ]
+  ])
 
+val MAX_SET_DEF = new_specification (
+  "MAX_SET_DEF", ["MAX_SET"],
+  SIMP_RULE bool_ss [AND_IMP_INTRO, GSYM RIGHT_EXISTS_IMP_THM,
+                     SKOLEM_THM] max_lemma);
 
+val MAX_SET_THM = store_thm(
+  "MAX_SET_THM",
+  ``(!e. MAX_SET {e} = e) /\
+    (!s. FINITE s ==> !e1 e2. MAX_SET (e1 INSERT e2 INSERT s) =
+                              MAX e1 (MAX_SET (e2 INSERT s)))``,
+  CONJ_TAC THENL [
+    GEN_TAC THEN
+    STRIP_ASSUME_TAC (SIMP_RULE bool_ss [FINITE_SING, NOT_INSERT_EMPTY,
+                                         IN_SING]
+                                (Q.SPEC `{e}` MAX_SET_DEF)),
+    REPEAT STRIP_TAC THEN
+    Q.ISPEC_THEN `e1 INSERT e2 INSERT s` MP_TAC MAX_SET_DEF THEN
+    ASM_SIMP_TAC bool_ss [FINITE_INSERT, NOT_INSERT_EMPTY,
+                          IN_INSERT, FORALL_AND_THM, DISJ_IMP_THM] THEN
+    STRIP_TAC THEN
+    Q.ISPEC_THEN `e2 INSERT s` MP_TAC MAX_SET_DEF THEN
+    ASM_SIMP_TAC bool_ss [FINITE_INSERT, NOT_INSERT_EMPTY,
+                          IN_INSERT, FORALL_AND_THM, DISJ_IMP_THM] THEN
+    STRIP_TAC THEN
+    Q.ABBREV_TAC `m1 = MAX_SET (e1 INSERT e2 INSERT s)` THEN
+    Q.ABBREV_TAC `m2 = MAX_SET (e2 INSERT s)` THEN
+    NTAC 2 (POP_ASSUM (K ALL_TAC)) THEN RES_TAC THEN
+    ASM_SIMP_TAC arith_ss [MAX_DEF]
+  ]);
 
+val MIN_SET_DEF = new_definition("MIN_SET_DEF", ``MIN_SET = $LEAST``);
+
+val MIN_SET_ELIM = store_thm(
+  "MIN_SET_ELIM",
+  ``!P Q. ~(P = {}) /\ (!x. (!y. y IN P ==> x <= y) /\ x IN P ==> Q x) ==>
+          Q (MIN_SET P)``,
+  REWRITE_TAC [MIN_SET_DEF] THEN REPEAT STRIP_TAC THEN
+  MATCH_MP_TAC LEAST_ELIM THEN CONJ_TAC THENL [
+    `?x. P x` by PROVE_TAC [SET_CASES, IN_INSERT, SPECIFICATION] THEN
+    PROVE_TAC [],
+    FULL_SIMP_TAC arith_ss [SPECIFICATION] THEN
+    PROVE_TAC [NOT_LESS]
+  ]);
+
+val MIN_SET_THM = store_thm(
+  "MIN_SET_THM",
+  ``(!e. MIN_SET {e} = e) /\
+    (!s e1 e2. MIN_SET (e1 INSERT e2 INSERT s) =
+               MIN e1 (MIN_SET (e2 INSERT s)))``,
+  CONJ_TAC THENL [
+    GEN_TAC THEN
+    Q.SPECL_THEN [`{e}`, `\x. x = e`] (MATCH_MP_TAC o BETA_RULE)
+                 MIN_SET_ELIM THEN
+    SIMP_TAC bool_ss [IN_INSERT, NOT_INSERT_EMPTY, DISJ_IMP_THM,
+                      NOT_IN_EMPTY],
+    REPEAT GEN_TAC THEN
+    Q.SPECL_THEN [`e1 INSERT e2 INSERT s`,
+                   `\x. x = MIN e1 (MIN_SET (e2 INSERT s))`]
+                 (MATCH_MP_TAC o BETA_RULE)
+                 MIN_SET_ELIM THEN
+    SIMP_TAC bool_ss [IN_INSERT, NOT_INSERT_EMPTY, DISJ_IMP_THM,
+                      FORALL_AND_THM] THEN
+    REPEAT STRIP_TAC THEN
+    Q.SPECL_THEN [`e2 INSERT s`, `\y. x = MIN e1 y`]
+                 (MATCH_MP_TAC o BETA_RULE)
+                 MIN_SET_ELIM THEN
+    SIMP_TAC bool_ss [IN_INSERT, NOT_INSERT_EMPTY, DISJ_IMP_THM,
+                      FORALL_AND_THM] THEN
+    REPEAT STRIP_TAC THEN RES_TAC THEN ASM_SIMP_TAC arith_ss [MIN_DEF]
+  ]);
 
 val _ = export_rewrites
     [
